Scattered cleanup

src/Dafny/jrnl.i.dfy
@@ -4,48 +4,60 @@ include "pow.dfy"
 Spec for sequential journal API, assuming we're using 2PL.
 */
 
-datatype Addr = Addr(blkno: nat, off: nat)
+type Blkno = nat
+datatype Addr = Addr(blkno: Blkno, off: nat)
 type byte = bv8
 type Object = array<byte>
 type Kind = k:int | 0 <= k <= 15
 
-function kindSize(k: Kind): nat {
+function objSize(obj: Object): nat
+{
+    obj.Length * 8
+}
+
+function kindSize(k: Kind): nat
+{
     pow_nonneg(2, k);
     pow(2,k)
 }
 
-function kindCount(k: Kind): nat {
+function kindCount(k: Kind): nat
+{
     pow_nonneg(2, 15-k);
     pow(2, 15-k)
 }
 
 lemma kindSize_and_kindCount_sensible(k: Kind)
-ensures kindSize(k) * kindCount(k) == 4096*8 {
+ensures kindSize(k) * kindCount(k) == 4096*8
+{
     assert 4096*8 == pow(2, 15);
     pow_plus(2, k, 15-k);
 }
 
 lemma kindSize_bounds(k: Kind)
-ensures kindSize(k) <= 4096*8 {
+ensures kindSize(k) <= 4096*8
+{
     pow_increasing(2, k, 15);
     assert pow(2,15) == 4096*8;
 }
 
-class {:autocontracts} Jrnl {
+class {:autocontracts} Jrnl
+{
     var data: map<Addr, Object>;
-    var kinds: map<nat, Kind>;
+    var kinds: map<Blkno, Kind>;
 
     predicate Valid() reads this {
         forall a :: a in data ==>
         && a.blkno in kinds
-        && data[a].Length*8 == kindSize(kinds[a.blkno])
+        && objSize(data[a]) == kindSize(kinds[a.blkno])
     }
 
-    constructor(kinds: map<nat, Kind>)
+    constructor(kinds: map<Blkno, Kind>)
     {
         this.kinds := kinds;
         // TODO: initializing data based on kinds is quite difficult
-        assume false;
+        new;
+        assume Valid();
     }
 
     function domain(): set<Addr>
@@ -69,6 +81,7 @@ class {:autocontracts} Jrnl {
     }
 }
 
+// TODO: couldn't figure out how to use autocontracts here
 class Txn {
     var jrnl: Jrnl;
 
@@ -80,34 +93,39 @@ class Txn {
         this.jrnl := jrnl;
     }
 
-    predicate Valid() reads {this,this.jrnl} + this.jrnl.Repr {
+    predicate Valid()
+    reads this, jrnl, jrnl.Repr
+    {
         this.jrnl.Valid()
     }
 
     method Read(a: Addr, sz: nat)
-    returns (o:Object)
+    returns (obj:Object)
     requires Valid()
+    modifies {}
     requires a in jrnl.domain()
     requires sz == jrnl.size(a)
-    modifies {}
-    ensures o.Length*8 == sz
+    ensures objSize(obj) == sz
     {
         return this.jrnl.data[a];
     }
 
     method Write(a: Addr, obj: Object)
+    requires Valid() ensures Valid()
     modifies jrnl
-    requires Valid()
-    ensures Valid()
     requires a in jrnl.domain()
-    requires obj.Length*8 == jrnl.size(a)
+    requires objSize(obj) == jrnl.size(a)
     //ensures jrnl.data == old(jrnl.data)[a:=obj]
     ensures jrnl.kinds == old(jrnl.kinds)
     {
         this.jrnl.data := this.jrnl.data[a:=obj];
     }
 
+    // NOTE: seems a bit wrong that Commit isn't necessary, but it's a result of
+    // modeling Reads and Writes as operating immediately (instead of somehow
+    // buffering their effects till this linearization point)
     method Commit()
+    modifies {}
     {
     }
 }
